complete verified C test, based on the unverified Rust example

src/cbor/pulse/det/vertest/c/CBORTest.fst
@@ -1,13 +1,15 @@
 module CBORTest
 open CBOR.Spec.Constants
 open CBOR.Pulse.API.Det.C
-module C = C
 open Pulse.Lib.Pervasives
 module A = Pulse.Lib.Array
 module SZ = FStar.SizeT
 module U8 = FStar.UInt8
 module SM = Pulse.Lib.SeqMatch.Util
 module Trade = Pulse.Lib.Trade.Util
+module Spec = CBOR.Spec.API.Format
+module I32 = FStar.Int32
+module S = Pulse.Lib.Slice
 
 inline_for_extraction
 noextract [@@noextract_to "krml"]
@@ -16,12 +18,166 @@ let letter (x: U8.t { 1 <= U8.v x /\ U8.v x <= 26 }) : U8.t =
 
 #push-options "--fuel 8 --z3rlimit 16"
 
+noextract [@@noextract_to "krml"]
+let spec_bar () : Pure (Seq.seq U8.t)
+  (requires True)
+  (ensures fun v ->
+    Seq.length v = 3 /\
+    Seq.index v 0 == letter 2uy /\
+    Seq.index v 1 == letter 1uy /\
+    Seq.index v 2 == letter 18uy /\
+    CBOR.Spec.API.UTF8.correct v
+  )
+= let v = Seq.seq_of_list [letter 2uy; letter 1uy; letter 18uy] in
+  CBOR.Spec.API.UTF8.ascii_is_utf8 v;
+  v
+
+noextract [@@noextract_to "krml"]
+let spec_test_on
+  (x: Spec.cbor)
+: Tot prop
+= match Spec.unpack x with
+  | Spec.CArray [_; _; xm] ->
+    begin match Spec.unpack xm with
+    | Spec.CMap m ->
+      begin match Spec.cbor_map_get m (Spec.pack (Spec.CString cbor_major_type_text_string (spec_bar ()))) with
+      | Some xv ->
+        begin match Spec.unpack xv with
+        | Spec.CInt64 ty v -> ty == cbor_major_type_neg_int64 /\ v == 42uL
+        | _ -> False
+        end
+      | _ -> False
+      end
+    | _ -> False
+    end
+  | _ -> False
+
+inline_for_extraction
+noextract [@@noextract_to "krml"]
+let exit_success : I32.t = 0l
+
+inline_for_extraction
+noextract [@@noextract_to "krml"]
+let exit_serialization_failure : I32.t = 1l
+
+inline_for_extraction
+noextract [@@noextract_to "krml"]
+let exit_impossible : I32.t = 2l
+
+#restart-solver
+```pulse
+fn test_on
+  (test: cbor_det_t)
+  (#p: perm)
+  (#v: Ghost.erased Spec.cbor)
+requires
+  cbor_det_match p test v **
+  pure (spec_test_on v)
+returns res: I32.t
+ensures
+  cbor_det_match p test v **
+  pure (res == exit_success)
+{
+  let ty = cbor_det_major_type () test;
+  if (ty <> cbor_major_type_array) {
+    exit_impossible
+  } else {
+    let len = cbor_det_get_array_length () test;
+    if (len <> 3uL) {
+      exit_impossible
+    } else {
+      let m = cbor_det_get_array_item () test 2uL;
+      let ty = cbor_det_major_type () m;
+      if (ty <> cbor_major_type_map) {
+        Trade.elim (cbor_det_match _ m _) _;
+        exit_impossible
+      } else {
+        let mut bar_payload = [| letter 2uy; 3sz |];
+        bar_payload.(1sz) <- letter 1uy;
+        bar_payload.(2sz) <- letter 18uy;
+        with s . assert (A.pts_to bar_payload s);
+        assert (pure (Seq.equal s (spec_bar ())));
+        let bar = cbor_det_mk_string_from_array () cbor_major_type_text_string bar_payload 3uL;
+        let ov = cbor_det_map_get () m bar;
+        with pm vm vk . assert (map_get_post cbor_det_match m pm vm vk ov);
+        Trade.elim (cbor_det_match _ bar _) _;
+        match ov {
+          None -> {
+            rewrite (map_get_post cbor_det_match m pm vm vk ov)
+              as (map_get_post_none cbor_det_match m pm vm vk);
+            unfold (map_get_post_none cbor_det_match m pm vm vk);
+            Trade.elim (cbor_det_match _ m _) _;
+            exit_impossible
+          }
+          Some v -> {
+            rewrite (map_get_post cbor_det_match m pm vm vk ov)
+              as (map_get_post_some cbor_det_match m pm vm vk v);
+            unfold (map_get_post_some cbor_det_match m pm vm vk v);
+            let ty = cbor_det_major_type () v;
+            if (ty <> cbor_major_type_neg_int64) {
+              Trade.elim (cbor_det_match _ v _) _;
+              Trade.elim (cbor_det_match _ m _) _;
+              exit_impossible
+            } else {
+              let i = cbor_det_read_uint64 () v;
+              Trade.elim (cbor_det_match _ v _) _;
+              Trade.elim (cbor_det_match _ m _) _;
+              if (i <> 42uL) {
+                exit_impossible
+              } else {
+                exit_success
+              }
+            }
+          }
+        }
+      }
+    }
+  }
+}
+```
+
+#pop-options
+
+let cbor_det_serialize_inj_strong
+  (x1 x2: Spec.cbor)
+  (y1 y2: Seq.seq U8.t)
+: Lemma
+  (requires (Spec.cbor_det_serialize x1 `Seq.append` y1 == Spec.cbor_det_serialize x2 `Seq.append` y2))
+  (ensures (x1 == x2 /\ y1 == y2))
+  [SMTPat (Spec.cbor_det_serialize x1 `Seq.append` y1); SMTPat (Spec.cbor_det_serialize x2 `Seq.append` y2)]
+= Spec.cbor_det_serialize_inj_strong x1 x2 y1 y2
+
+inline_for_extraction
+noextract [@@noextract_to "krml"]
+let res_post
+  (res: I32.t)
+: Tot prop
+= res == exit_success \/ res == exit_serialization_failure
+
+inline_for_extraction
+noextract [@@noextract_to "krml"]
+let res_t = (res: I32.t { res_post res })
+
+inline_for_extraction
+noextract [@@noextract_to "krml"]
+let intro_res_post_success : res_t = exit_success
+
+inline_for_extraction
+noextract [@@noextract_to "krml"]
+let intro_res_post_serialization_failure : res_t = exit_serialization_failure
+
+inline_for_extraction
+noextract [@@noextract_to "krml"]
+let intro_res_post_impossible (_: squash False) : res_t = exit_impossible
+
+#push-options "--fuel 8 --z3rlimit 128"
+
 #restart-solver
 ```pulse
 fn main (_: unit)
 requires emp
-returns res: C.exit_code
-ensures pure (res == C.EXIT_SUCCESS)
+returns res: res_t
+ensures emp
 {
   Classical.forall_intro (Classical.move_requires CBOR.Spec.API.UTF8.ascii_is_utf8);
   let mut foo0 = [| letter 6uy; 3sz |];
@@ -39,6 +195,7 @@ ensures pure (res == C.EXIT_SUCCESS)
   bar0.(2sz) <- letter 18uy;
   with bar_v . assert (A.pts_to bar0 bar_v);
   assert (pure (~ (Seq.index foo_v 0 == Seq.index bar_v 0))); // necessary to prove that foo <> bar
+  assert (pure (Seq.equal bar_v (spec_bar ())));
   let bar = cbor_det_mk_string_from_array () cbor_major_type_text_string bar0 3uL;
   let i42 = cbor_det_mk_int64' cbor_major_type_neg_int64 42uL;
   let bar_i42 = cbor_det_mk_map_entry () bar i42;
@@ -87,8 +244,78 @@ ensures pure (res == C.EXIT_SUCCESS)
   Trade.trans_concl_l _ (cbor_det_match 1.0R array_entry0 _) _ _;
   let test = cbor_det_mk_array_from_array' array 3uL _;
   Trade.trans_concl_r (cbor_det_match _ test _) _ _ _;
-
-  Trade.elim _ _;
-  C.EXIT_SUCCESS
+  let res = test_on test;
+  if (res <> exit_success) {
+    Trade.elim (cbor_det_match _ test _) _;
+    intro_res_post_impossible ()
+  } else {
+    let max_size = 32sz;
+    let size = cbor_det_size test max_size;
+    if (size = 0sz) {
+      Trade.elim (cbor_det_match _ test _) _;
+      intro_res_post_serialization_failure // I cannot prove that this case cannot happen
+    } else {
+      let mut output_bytes = [| 0xFFuy; max_size |];
+      let out1 = S.from_array output_bytes max_size;
+      S.pts_to_len out1;
+      let size' = cbor_det_serialize test out1;
+      if (size' <> size) {
+        S.to_array out1;
+        Trade.elim (cbor_det_match _ test _) _;
+        intro_res_post_impossible ()
+      } else {
+        let size' = cbor_det_validate out1;
+        if (size' <> size) {
+          S.to_array out1;
+          Trade.elim (cbor_det_match _ test _) _;
+          intro_res_post_impossible ()
+        } else {
+          with w . assert (pts_to out1 w);
+          Seq.lemma_split w (SZ.v size');
+          let test1 = cbor_det_parse out1 size';
+          let b = cbor_det_equal () test test1;
+          if (not b) {
+            Trade.elim (cbor_det_match _ test1 _) _;
+            S.to_array out1;
+            Trade.elim (cbor_det_match _ test _) _;
+            intro_res_post_impossible ()
+          } else {
+            let res = test_on test1;
+            Trade.elim (cbor_det_match _ test1 _) _;
+            if (res <> exit_success) {
+              S.to_array out1;
+              Trade.elim (cbor_det_match _ test _) _;
+              intro_res_post_impossible ()
+            } else {
+              let Mktuple2 out2 out3 = S.split out1 size';
+              Seq.append_empty_r (Seq.slice w 0 (SZ.v size'));
+              let test2 = cbor_det_parse out2 size';
+              let b = cbor_det_equal () test test2;
+              if (not b) {
+                 Trade.elim (cbor_det_match _ test2 _) _;
+                 S.join out2 out3 out1;
+                 S.to_array out1;
+                 Trade.elim (cbor_det_match _ test _) _;
+                 intro_res_post_impossible ()
+              } else {
+                let res = test_on test2;
+                Trade.elim (cbor_det_match _ test2 _) _;
+                S.join out2 out3 out1;
+                S.to_array out1;
+                Trade.elim (cbor_det_match _ test _) _;
+                if (res <> exit_success) {
+                   intro_res_post_impossible ()
+                } else {
+                  intro_res_post_success
+                }
+              }
+            }
+          }
+        }
+      }
+    }
+  }
 }
 ```
+
+#pop-options
